Move Afix definition out of the way

Launchbury/ArityAnalysis.thy
@@ -14,6 +14,34 @@ lemma Aexp'_simps[simp]:
   "Aexp' e \<cdot> (up\<cdot>n) = Aexp e \<cdot> n"
   unfolding Aexp'_def by simp_all
 
+lemma env_restr_join:
+  fixes m1 m2 :: "'a::type \<Rightarrow> 'b::{Finite_Join_cpo,pcpo}"
+  shows "(m1 \<squnion> m2) f|` S = (m1 f|` S) \<squnion> (m2 f|` S )"
+  by (auto simp add: env_restr_def)
+
+lemma join_env_restr_UNIV:
+  fixes m :: "'a::type \<Rightarrow> 'b::{Finite_Join_cpo,pcpo}"
+  shows "S1 \<union> S2 = UNIV \<Longrightarrow> (m f|` S1) \<squnion> (m f|` S2) = m"
+  by (fastforce simp add: env_restr_def)
+
+definition inc_bot :: "Arity\<^sub>\<bottom> \<rightarrow> Arity\<^sub>\<bottom>" ("inc\<^sub>\<bottom>") where "inc_bot = fup\<cdot>(up oo inc)"
+
+lemma inc_bot_simps[simp]:
+  "inc\<^sub>\<bottom>\<cdot>\<bottom>=\<bottom>"
+  "inc\<^sub>\<bottom>\<cdot>(up\<cdot>n)=up\<cdot>(inc\<cdot>n)"
+  unfolding inc_bot_def by simp_all
+
+end
+
+lemma Aexp'_eqvt[eqvt]: "\<pi> \<bullet> (ArityAnalysis.Aexp' Aexp e) = ArityAnalysis.Aexp' (\<pi> \<bullet> Aexp) (\<pi> \<bullet> e)"
+  unfolding ArityAnalysis.Aexp'_def
+  by perm_simp rule
+
+subsection {* Lifting arity analysis to heaps *}
+
+context ArityAnalysis
+begin
+
 definition ABind :: "var \<Rightarrow> exp \<Rightarrow> (AEnv \<rightarrow> AEnv)"
   where "ABind v e = (\<Lambda> ae. Aexp' e \<cdot> (ae v))"
 
@@ -66,70 +94,6 @@ next
   finally show "ae \<sqsubseteq> ABinds ((v, e) # \<Gamma>)\<cdot>ae" by this simp
 qed
 
-definition Afix ::  "heap \<Rightarrow> (AEnv \<rightarrow> AEnv)"
-  where "Afix \<Gamma> = (\<Lambda> ae. (\<mu>  ae'. ABinds \<Gamma> \<cdot> ae' \<squnion> ae))"
-
-lemma Afix_eq: "Afix \<Gamma> \<cdot> ae = (\<mu>  ae'. (ABinds \<Gamma> \<cdot> ae') \<squnion> ae)"
-  unfolding Afix_def by simp
-
-lemma Afix_strict[simp]: "Afix \<Gamma> \<cdot> \<bottom> = \<bottom>"
-  unfolding Afix_eq
-  by (rule fix_eqI) auto
-
-lemma Afix_least_below: "ABinds \<Gamma> \<cdot> ae' \<sqsubseteq> ae' \<Longrightarrow> ae \<sqsubseteq> ae' \<Longrightarrow> Afix \<Gamma> \<cdot> ae \<sqsubseteq> ae'"
-  unfolding Afix_eq
-  by (auto intro: fix_least_below)
-
-lemma Afix_unroll: "Afix \<Gamma>\<cdot>ae = ABinds \<Gamma> \<cdot> (Afix \<Gamma>\<cdot>ae) \<squnion> ae"
-  unfolding Afix_eq
-  apply (subst fix_eq)
-  by simp
-
-lemma Abinds_below_Afix: "ABinds \<Delta> \<sqsubseteq> Afix \<Delta>"
-  apply (rule cfun_belowI)
-  apply (simp add: Afix_eq)
-  apply (subst fix_eq, simp)
-  apply (rule below_trans[OF _ join_above1])
-  apply (rule monofun_cfun_arg)
-  apply (subst fix_eq, simp)
-  done
-
-lemma Afix_above_arg: "ae \<sqsubseteq> Afix \<Gamma> \<cdot> ae"
-  by (metis (hide_lams, no_types) Abinds_below_Afix ArityAnalysis.ABinds_above_arg below_refl box_below monofun_cfun_fun)
-
-
-lemma Abinds_Afix[simp]: "ABinds \<Gamma>\<cdot>(Afix \<Gamma>\<cdot>ae) = Afix \<Gamma>\<cdot>ae"
-  unfolding Afix_eq
-  apply (subst fix_eq) back apply simp
-  apply (rule below_trans[OF ABinds_above_arg monofun_cfun_arg])
-  apply (subst fix_eq) apply simp
-  done
-
-lemma Afix_reorder: "map_of \<Gamma> = map_of \<Delta> \<Longrightarrow> Afix \<Gamma> = Afix \<Delta>"
-  by (intro cfun_eqI)(simp add: Afix_eq cong: Abinds_reorder)
-
-lemma env_restr_join:
-  fixes m1 m2 :: "'a::type \<Rightarrow> 'b::{Finite_Join_cpo,pcpo}"
-  shows "(m1 \<squnion> m2) f|` S = (m1 f|` S) \<squnion> (m2 f|` S )"
-  by (auto simp add: env_restr_def)
-
-lemma join_env_restr_UNIV:
-  fixes m :: "'a::type \<Rightarrow> 'b::{Finite_Join_cpo,pcpo}"
-  shows "S1 \<union> S2 = UNIV \<Longrightarrow> (m f|` S1) \<squnion> (m f|` S2) = m"
-  by (fastforce simp add: env_restr_def)
-
-lemma Afix_repeat_singleton: "(\<mu> xa. Afix \<Gamma>\<cdot>(AE_singleton x\<cdot>(n \<squnion> xa x) \<squnion> ae)) = Afix \<Gamma>\<cdot>(AE_singleton x\<cdot>n \<squnion> ae)"
-  apply (rule below_antisym)
-  defer
-  apply (subst fix_eq, simp)
-  apply (intro monofun_cfun_arg join_mono below_refl join_above1)
-
-  apply (rule fix_least_below, simp)
-  apply (rule Afix_least_below, simp)
-  apply (intro join_below below_refl iffD2[OF AE_singleton_below_iff] below_trans[OF _ fun_belowD[OF Afix_above_arg]]  below_trans[OF _ Afix_above_arg] join_above2)
-  apply simp
-  done
-
 lemma Abinds_join_fresh: "ae' ` (domA \<Delta>) \<subseteq> {\<bottom>} \<Longrightarrow>  ABinds \<Delta>\<cdot>(ae \<squnion> ae') = (ABinds \<Delta>\<cdot>ae) \<squnion> ae'"
 proof (induct \<Delta> rule: ABinds.induct)
   case 1 thus ?case by simp
@@ -143,20 +107,7 @@ next
   ultimately
   show "ABinds ((v, e) # \<Delta>)\<cdot>(ae \<squnion> ae') = ABinds ((v, e) # \<Delta>)\<cdot>ae \<squnion> ae'"
     by simp
-qed  
-
-lemma Afix_join_fresh: "ae' ` (domA \<Delta>) \<subseteq> {\<bottom>}  \<Longrightarrow>  Afix \<Delta>\<cdot>(ae \<squnion> ae') = (Afix \<Delta>\<cdot>ae) \<squnion> ae'"
-  apply (rule below_antisym)
-  apply (rule Afix_least_below)
-  apply (simp add: Abinds_join_fresh)
-  apply (rule join_below)
-  apply (rule below_trans[OF Afix_above_arg join_above1])
-  apply (rule join_above2)
-  apply (rule join_below[OF monofun_cfun_arg [OF join_above1]])
-  apply (rule below_trans[OF join_above2 Afix_above_arg])
-  done
-
-
+qed
 
 lemma ABinds_restr_fresh:
   assumes "atom ` S \<sharp>* \<Gamma>"
@@ -170,41 +121,11 @@ lemma ABinds_restr_fresh:
   apply rule
   done
 
-
-lemma Afix_restr_fresh:
-  assumes "atom ` S \<sharp>* \<Gamma>"
-  shows "Afix \<Gamma>\<cdot>ae f|` (- S) = Afix \<Gamma>\<cdot>(ae  f|` (- S)) f|` (- S)"
-unfolding Afix_eq
-proof (rule parallel_fix_ind[where P = "\<lambda> x y . x f|` (- S) = y  f|` (- S)"])
-  case goal1 show ?case by simp
-next
-  case goal2 show ?case..
-next
-  case (goal3 aeL aeR)
-  have "(ABinds \<Gamma>\<cdot>aeL \<squnion> ae) f|` (- S) = ABinds \<Gamma>\<cdot>aeL  f|` (- S) \<squnion> ae  f|` (- S)" by (simp add: env_restr_join)
-  also have "\<dots> = ABinds \<Gamma>\<cdot>(aeL  f|` (- S)) f|` (- S) \<squnion> ae  f|` (- S)" by (rule arg_cong[OF ABinds_restr_fresh[OF assms]])
-  also have "\<dots> = ABinds \<Gamma>\<cdot>(aeR  f|` (- S)) f|` (- S) \<squnion> ae  f|` (- S)" unfolding goal3..
-  also have "\<dots> = ABinds \<Gamma>\<cdot>aeR f|` (- S) \<squnion> ae  f|` (- S)" by (rule arg_cong[OF ABinds_restr_fresh[OF assms, symmetric]])
-  also have "\<dots> = (ABinds \<Gamma>\<cdot>aeR \<squnion> ae f|` (- S)) f|` (- S)" by (simp add: env_restr_join)
-  finally show ?case by simp
-qed
-
 lemma ABinds_restr:
   assumes "domA \<Gamma> \<subseteq> S"
   shows "ABinds \<Gamma>\<cdot>ae f|` S = ABinds \<Gamma>\<cdot>(ae  f|` S) f|` S"
   using assms
   by (induction \<Gamma> rule:ABinds.induct) (fastforce simp del: fun_meet_simp simp add: env_restr_join)+
-
-lemma Afix_restr:
-  assumes "domA \<Gamma> \<subseteq> S"
-  shows "Afix \<Gamma>\<cdot>ae f|` S = Afix \<Gamma>\<cdot>(ae  f|` S) f|` S"
-  unfolding Afix_eq
-  apply (rule parallel_fix_ind[where P = "\<lambda> x y . x f|`S = y  f|` S"])
-  apply simp
-  apply rule
-  apply (auto   simp add: env_restr_join)
-  apply (metis  ABinds_restr[OF assms, symmetric])
-  done
 
 lemma ABinds_restr_subst:
   assumes "\<And> x' e a. (x',e) \<in> set \<Gamma> \<Longrightarrow> Aexp e[x::=y]\<cdot>a f|` S = Aexp e\<cdot>a f|` S"
@@ -220,76 +141,8 @@ lemma ABinds_restr_subst:
   apply (auto dest:  set_mp[OF set_delete_subset])
   done
 
-lemma Afix_restr_subst':
-  assumes "\<And> x' e a. (x',e) \<in> set \<Gamma> \<Longrightarrow> Aexp e[x::=y]\<cdot>a f|` S = Aexp e\<cdot>a f|` S"
-  assumes "x \<notin> S"
-  assumes "y \<notin> S"
-  assumes "domA \<Gamma> \<subseteq> S"
-  shows "Afix \<Gamma>[x::h=y]\<cdot>ae f|` S = Afix \<Gamma>\<cdot>(ae f|` S) f|` S"
-  unfolding Afix_eq
-  apply (rule parallel_fix_ind[where P = "\<lambda> x y . x f|`S = y  f|` S"])
-  apply simp
-  apply rule
-  apply (auto   simp add: env_restr_join)
-  apply (subst ABinds_restr_subst[OF assms]) apply assumption
-  apply (subst ABinds_restr[OF assms(4)]) back
-  apply simp
-  done
-
- 
-lemma Afix_subst_approx:
-  assumes "\<And> v n. v \<in> domA \<Gamma> \<Longrightarrow> Aexp (the (map_of \<Gamma> v))[y::=x]\<cdot>n \<sqsubseteq> (Aexp (the (map_of \<Gamma> v))\<cdot>n)(y := \<bottom>, x := up\<cdot>0)"
-  assumes "x \<notin> domA \<Gamma>"
-  assumes "y \<notin> domA \<Gamma>"
-  shows "Afix \<Gamma>[y::h= x]\<cdot>(ae(y := \<bottom>, x := up\<cdot>0)) \<sqsubseteq> (Afix \<Gamma>\<cdot>ae)(y := \<bottom>, x := up\<cdot>0)"
-unfolding Afix_eq
-proof (rule parallel_fix_ind[where P = "\<lambda> aeL aeR . aeL \<sqsubseteq> aeR(y := \<bottom>, x := up\<cdot>0)"])
-  case goal1 show ?case by simp
-next
-  case goal2 show ?case..
-next
-  case (goal3 aeL aeR)
-  hence "ABinds \<Gamma>[y::h=x]\<cdot>aeL \<sqsubseteq> ABinds \<Gamma>[y::h=x]\<cdot>(aeR (y := \<bottom>, x := up\<cdot>0))" by (rule monofun_cfun_arg)
-  also have "\<dots>  \<sqsubseteq> (ABinds \<Gamma>\<cdot>aeR)(y := \<bottom>, x := up\<cdot>0)"
-  using assms
-  proof(induction  rule: ABinds.induct)
-  case goal1 thus ?case by simp
-  next
-  case (goal2 v e \<Gamma>)
-    have "\<And> n. Aexp e[y::=x]\<cdot>n \<sqsubseteq> (Aexp e\<cdot>n)(y := \<bottom>, x := up\<cdot>0)" using goal2(2)[where v = v] by auto
-    hence IH1: "\<And> n. Aexp' e[y::=x]\<cdot>n \<sqsubseteq> (Aexp' e\<cdot>n)(y := \<bottom>, x := up\<cdot>0)" unfolding Aexp'_def by (case_tac n) auto
-
-    have "ABinds (delete v \<Gamma>)[y::h=x]\<cdot>(aeR(y := \<bottom>, x := up\<cdot>0)) \<sqsubseteq> (ABinds (delete v \<Gamma>)\<cdot>aeR)(y := \<bottom>, x := up\<cdot>0)"
-      apply (rule goal2) using goal2(2,3,4) by fastforce+
-    hence IH2: "ABinds (delete v \<Gamma>[y::h=x])\<cdot>(aeR(y := \<bottom>, x := up\<cdot>0)) \<sqsubseteq> (ABinds (delete v \<Gamma>)\<cdot>aeR)(y := \<bottom>, x := up\<cdot>0)"
-       unfolding subst_heap_delete.
-    
-    have [simp]: "(aeR(y := \<bottom>, x := up\<cdot>0)) v = aeR v" using goal2(3,4) by auto
-   
-    show ?case by (simp del: fun_upd_apply) (rule join_mono[OF IH1 IH2])
-  qed
-  finally
-  have "ABinds \<Gamma>[y::h=x]\<cdot>aeL \<sqsubseteq> (ABinds \<Gamma>\<cdot>aeR)(y := \<bottom>, x := up\<cdot>0)" by this simp
-  thus ?case by (simp add: join_mono)
-qed
-
-
-definition Acomplete :: "heap \<Rightarrow> exp \<Rightarrow> (AEnv \<rightarrow> AEnv) \<Rightarrow> Arity \<rightarrow> AEnv"
-  where "Acomplete \<Gamma> e F = (\<Lambda> a. (\<mu> ae. ABinds \<Gamma> \<squnion> F) \<cdot> (Aexp e \<cdot> a))"
-
-definition inc_bot :: "Arity\<^sub>\<bottom> \<rightarrow> Arity\<^sub>\<bottom>" ("inc\<^sub>\<bottom>") where "inc_bot = fup\<cdot>(up oo inc)"
-
-lemma inc_bot_simps[simp]:
-  "inc\<^sub>\<bottom>\<cdot>\<bottom>=\<bottom>"
-  "inc\<^sub>\<bottom>\<cdot>(up\<cdot>n)=up\<cdot>(inc\<cdot>n)"
-  unfolding inc_bot_def by simp_all
-
 end
 
-
-lemma Aexp'_eqvt[eqvt]: "\<pi> \<bullet> (ArityAnalysis.Aexp' Aexp e) = ArityAnalysis.Aexp' (\<pi> \<bullet> Aexp) (\<pi> \<bullet> e)"
-  unfolding ArityAnalysis.Aexp'_def
-  by perm_simp rule
 
 lemma ABind_eqvt[eqvt]: "\<pi> \<bullet> (ArityAnalysis.ABind Aexp v e) = ArityAnalysis.ABind (\<pi> \<bullet> Aexp) (\<pi> \<bullet> v) (\<pi> \<bullet> e)"
   unfolding ArityAnalysis.ABind_def
@@ -302,10 +155,6 @@ lemma ABinds_eqvt[eqvt]: "\<pi> \<bullet> (ArityAnalysis.ABinds Aexp \<Gamma>) =
   apply perm_simp
   apply simp
   done
-
-lemma Afix_eqvt[eqvt]: "\<pi> \<bullet> (ArityAnalysis.Afix Aexp \<Gamma>) = ArityAnalysis.Afix  (\<pi> \<bullet> Aexp) (\<pi> \<bullet> \<Gamma>)"
-  unfolding ArityAnalysis.Afix_def
-  by perm_simp (simp add: Abs_cfun_eqvt)
 
 lemma Abinds_cong[fundef_cong]:
   "\<lbrakk> (\<And> e. e \<in> snd ` set heap2 \<Longrightarrow> aexp1 e = aexp2 e) ; heap1 = heap2 \<rbrakk>
@@ -322,10 +171,5 @@ case (goal2  v e as heap2)
   note goal2(1)[OF this refl] with goal2
   show ?case by (auto simp add: ArityAnalysis.ABinds.simps ArityAnalysis.ABind_def ArityAnalysis.Aexp'_def)
 qed
-
-lemma Afix_cong[fundef_cong]:
-  "\<lbrakk> (\<And> e. e \<in> snd ` set heap2 \<Longrightarrow> aexp1 e = aexp2 e); heap1 = heap2 \<rbrakk>
-      \<Longrightarrow> ArityAnalysis.Afix aexp1 heap1 = ArityAnalysis.Afix aexp2 heap2"
-   unfolding ArityAnalysis.Afix_def by (metis Abinds_cong)
 
 end
