Launchbury/ArityAnalysisFix.thy
@@ -1,0 +1,436 @@
+theory ArityAnalysisFix
+imports ArityAnalysis ArityCorrect
+begin
+
+context ArityAnalysis
+begin
+
+definition Afix ::  "heap \<Rightarrow> (AEnv \<rightarrow> AEnv)"
+  where "Afix \<Gamma> = (\<Lambda> ae. (\<mu>  ae'. ABinds \<Gamma> \<cdot> ae' \<squnion> ae))"
+
+lemma Afix_eq: "Afix \<Gamma> \<cdot> ae = (\<mu>  ae'. (ABinds \<Gamma> \<cdot> ae') \<squnion> ae)"
+  unfolding Afix_def by simp
+
+lemma Afix_strict[simp]: "Afix \<Gamma> \<cdot> \<bottom> = \<bottom>"
+  unfolding Afix_eq
+  by (rule fix_eqI) auto
+
+lemma Afix_least_below: "ABinds \<Gamma> \<cdot> ae' \<sqsubseteq> ae' \<Longrightarrow> ae \<sqsubseteq> ae' \<Longrightarrow> Afix \<Gamma> \<cdot> ae \<sqsubseteq> ae'"
+  unfolding Afix_eq
+  by (auto intro: fix_least_below)
+
+lemma Afix_unroll: "Afix \<Gamma>\<cdot>ae = ABinds \<Gamma> \<cdot> (Afix \<Gamma>\<cdot>ae) \<squnion> ae"
+  unfolding Afix_eq
+  apply (subst fix_eq)
+  by simp
+
+lemma Abinds_below_Afix: "ABinds \<Delta> \<sqsubseteq> Afix \<Delta>"
+  apply (rule cfun_belowI)
+  apply (simp add: Afix_eq)
+  apply (subst fix_eq, simp)
+  apply (rule below_trans[OF _ join_above1])
+  apply (rule monofun_cfun_arg)
+  apply (subst fix_eq, simp)
+  done
+
+lemma Afix_above_arg: "ae \<sqsubseteq> Afix \<Gamma> \<cdot> ae"
+  by (metis (hide_lams, no_types) Abinds_below_Afix ArityAnalysis.ABinds_above_arg below_refl box_below monofun_cfun_fun)
+
+
+lemma Abinds_Afix[simp]: "ABinds \<Gamma>\<cdot>(Afix \<Gamma>\<cdot>ae) = Afix \<Gamma>\<cdot>ae"
+  unfolding Afix_eq
+  apply (subst fix_eq) back apply simp
+  apply (rule below_trans[OF ABinds_above_arg monofun_cfun_arg])
+  apply (subst fix_eq) apply simp
+  done
+
+lemma Afix_reorder: "map_of \<Gamma> = map_of \<Delta> \<Longrightarrow> Afix \<Gamma> = Afix \<Delta>"
+  by (intro cfun_eqI)(simp add: Afix_eq cong: Abinds_reorder)
+
+lemma Afix_repeat_singleton: "(\<mu> xa. Afix \<Gamma>\<cdot>(AE_singleton x\<cdot>(n \<squnion> xa x) \<squnion> ae)) = Afix \<Gamma>\<cdot>(AE_singleton x\<cdot>n \<squnion> ae)"
+  apply (rule below_antisym)
+  defer
+  apply (subst fix_eq, simp)
+  apply (intro monofun_cfun_arg join_mono below_refl join_above1)
+
+  apply (rule fix_least_below, simp)
+  apply (rule Afix_least_below, simp)
+  apply (intro join_below below_refl iffD2[OF AE_singleton_below_iff] below_trans[OF _ fun_belowD[OF Afix_above_arg]]  below_trans[OF _ Afix_above_arg] join_above2)
+  apply simp
+  done
+
+lemma Afix_join_fresh: "ae' ` (domA \<Delta>) \<subseteq> {\<bottom>}  \<Longrightarrow>  Afix \<Delta>\<cdot>(ae \<squnion> ae') = (Afix \<Delta>\<cdot>ae) \<squnion> ae'"
+  apply (rule below_antisym)
+  apply (rule Afix_least_below)
+  apply (simp add: Abinds_join_fresh)
+  apply (rule join_below)
+  apply (rule below_trans[OF Afix_above_arg join_above1])
+  apply (rule join_above2)
+  apply (rule join_below[OF monofun_cfun_arg [OF join_above1]])
+  apply (rule below_trans[OF join_above2 Afix_above_arg])
+  done
+
+
+lemma Afix_restr_fresh:
+  assumes "atom ` S \<sharp>* \<Gamma>"
+  shows "Afix \<Gamma>\<cdot>ae f|` (- S) = Afix \<Gamma>\<cdot>(ae  f|` (- S)) f|` (- S)"
+unfolding Afix_eq
+proof (rule parallel_fix_ind[where P = "\<lambda> x y . x f|` (- S) = y  f|` (- S)"])
+  case goal1 show ?case by simp
+next
+  case goal2 show ?case..
+next
+  case (goal3 aeL aeR)
+  have "(ABinds \<Gamma>\<cdot>aeL \<squnion> ae) f|` (- S) = ABinds \<Gamma>\<cdot>aeL  f|` (- S) \<squnion> ae  f|` (- S)" by (simp add: env_restr_join)
+  also have "\<dots> = ABinds \<Gamma>\<cdot>(aeL  f|` (- S)) f|` (- S) \<squnion> ae  f|` (- S)" by (rule arg_cong[OF ABinds_restr_fresh[OF assms]])
+  also have "\<dots> = ABinds \<Gamma>\<cdot>(aeR  f|` (- S)) f|` (- S) \<squnion> ae  f|` (- S)" unfolding goal3..
+  also have "\<dots> = ABinds \<Gamma>\<cdot>aeR f|` (- S) \<squnion> ae  f|` (- S)" by (rule arg_cong[OF ABinds_restr_fresh[OF assms, symmetric]])
+  also have "\<dots> = (ABinds \<Gamma>\<cdot>aeR \<squnion> ae f|` (- S)) f|` (- S)" by (simp add: env_restr_join)
+  finally show ?case by simp
+qed
+
+lemma Afix_restr:
+  assumes "domA \<Gamma> \<subseteq> S"
+  shows "Afix \<Gamma>\<cdot>ae f|` S = Afix \<Gamma>\<cdot>(ae  f|` S) f|` S"
+  unfolding Afix_eq
+  apply (rule parallel_fix_ind[where P = "\<lambda> x y . x f|`S = y  f|` S"])
+  apply simp
+  apply rule
+  apply (auto   simp add: env_restr_join)
+  apply (metis  ABinds_restr[OF assms, symmetric])
+  done
+
+lemma Afix_restr_subst':
+  assumes "\<And> x' e a. (x',e) \<in> set \<Gamma> \<Longrightarrow> Aexp e[x::=y]\<cdot>a f|` S = Aexp e\<cdot>a f|` S"
+  assumes "x \<notin> S"
+  assumes "y \<notin> S"
+  assumes "domA \<Gamma> \<subseteq> S"
+  shows "Afix \<Gamma>[x::h=y]\<cdot>ae f|` S = Afix \<Gamma>\<cdot>(ae f|` S) f|` S"
+  unfolding Afix_eq
+  apply (rule parallel_fix_ind[where P = "\<lambda> x y . x f|`S = y  f|` S"])
+  apply simp
+  apply rule
+  apply (auto   simp add: env_restr_join)
+  apply (subst ABinds_restr_subst[OF assms]) apply assumption
+  apply (subst ABinds_restr[OF assms(4)]) back
+  apply simp
+  done
+
+ 
+lemma Afix_subst_approx:
+  assumes "\<And> v n. v \<in> domA \<Gamma> \<Longrightarrow> Aexp (the (map_of \<Gamma> v))[y::=x]\<cdot>n \<sqsubseteq> (Aexp (the (map_of \<Gamma> v))\<cdot>n)(y := \<bottom>, x := up\<cdot>0)"
+  assumes "x \<notin> domA \<Gamma>"
+  assumes "y \<notin> domA \<Gamma>"
+  shows "Afix \<Gamma>[y::h= x]\<cdot>(ae(y := \<bottom>, x := up\<cdot>0)) \<sqsubseteq> (Afix \<Gamma>\<cdot>ae)(y := \<bottom>, x := up\<cdot>0)"
+unfolding Afix_eq
+proof (rule parallel_fix_ind[where P = "\<lambda> aeL aeR . aeL \<sqsubseteq> aeR(y := \<bottom>, x := up\<cdot>0)"])
+  case goal1 show ?case by simp
+next
+  case goal2 show ?case..
+next
+  case (goal3 aeL aeR)
+  hence "ABinds \<Gamma>[y::h=x]\<cdot>aeL \<sqsubseteq> ABinds \<Gamma>[y::h=x]\<cdot>(aeR (y := \<bottom>, x := up\<cdot>0))" by (rule monofun_cfun_arg)
+  also have "\<dots>  \<sqsubseteq> (ABinds \<Gamma>\<cdot>aeR)(y := \<bottom>, x := up\<cdot>0)"
+  using assms
+  proof(induction  rule: ABinds.induct)
+  case goal1 thus ?case by simp
+  next
+  case (goal2 v e \<Gamma>)
+    have "\<And> n. Aexp e[y::=x]\<cdot>n \<sqsubseteq> (Aexp e\<cdot>n)(y := \<bottom>, x := up\<cdot>0)" using goal2(2)[where v = v] by auto
+    hence IH1: "\<And> n. Aexp' e[y::=x]\<cdot>n \<sqsubseteq> (Aexp' e\<cdot>n)(y := \<bottom>, x := up\<cdot>0)" unfolding Aexp'_def by (case_tac n) auto
+
+    have "ABinds (delete v \<Gamma>)[y::h=x]\<cdot>(aeR(y := \<bottom>, x := up\<cdot>0)) \<sqsubseteq> (ABinds (delete v \<Gamma>)\<cdot>aeR)(y := \<bottom>, x := up\<cdot>0)"
+      apply (rule goal2) using goal2(2,3,4) by fastforce+
+    hence IH2: "ABinds (delete v \<Gamma>[y::h=x])\<cdot>(aeR(y := \<bottom>, x := up\<cdot>0)) \<sqsubseteq> (ABinds (delete v \<Gamma>)\<cdot>aeR)(y := \<bottom>, x := up\<cdot>0)"
+       unfolding subst_heap_delete.
+    
+    have [simp]: "(aeR(y := \<bottom>, x := up\<cdot>0)) v = aeR v" using goal2(3,4) by auto
+   
+    show ?case by (simp del: fun_upd_apply) (rule join_mono[OF IH1 IH2])
+  qed
+  finally
+  have "ABinds \<Gamma>[y::h=x]\<cdot>aeL \<sqsubseteq> (ABinds \<Gamma>\<cdot>aeR)(y := \<bottom>, x := up\<cdot>0)" by this simp
+  thus ?case by (simp add: join_mono)
+qed
+
+end
+
+lemma Afix_eqvt[eqvt]: "\<pi> \<bullet> (ArityAnalysis.Afix Aexp \<Gamma>) = ArityAnalysis.Afix  (\<pi> \<bullet> Aexp) (\<pi> \<bullet> \<Gamma>)"
+  unfolding ArityAnalysis.Afix_def
+  by perm_simp (simp add: Abs_cfun_eqvt)
+
+
+lemma Afix_cong[fundef_cong]:
+  "\<lbrakk> (\<And> e. e \<in> snd ` set heap2 \<Longrightarrow> aexp1 e = aexp2 e); heap1 = heap2 \<rbrakk>
+      \<Longrightarrow> ArityAnalysis.Afix aexp1 heap1 = ArityAnalysis.Afix aexp2 heap2"
+   unfolding ArityAnalysis.Afix_def by (metis Abinds_cong)
+
+context EdomArityAnalysis
+begin
+lemma Afix_edom: "edom (Afix \<Gamma> \<cdot> ae) \<subseteq> fv \<Gamma> \<union> edom ae"
+  unfolding Afix_eq
+  by (rule fix_ind[where P = "\<lambda> ae' . edom ae' \<subseteq> fv \<Gamma> \<union> edom ae"] )
+     (auto dest: set_mp[OF ABinds_edom])
+end
+
+locale CorrectArityAnalysisAfix = CorrectArityAnalysis + 
+  assumes Aexp_Let: "Afix as\<cdot>(Aexp e\<cdot>n) f|` (- domA as) \<sqsubseteq> Aexp (Let as e)\<cdot>n"
+
+context CorrectArityAnalysis
+begin
+
+lemma Afix_lookup_fresh:
+  assumes "atom v \<sharp> \<Gamma>"
+  shows "(Afix \<Gamma>\<cdot>ae) v = ae v"
+  apply (rule below_antisym)
+  apply (subst Afix_eq)
+  apply (rule fix_ind[where  P = "\<lambda> ae'. ae' v \<sqsubseteq> ae v"])
+  apply (auto simp add: ABinds_lookup_fresh[OF assms] fun_belowD[OF Afix_above_arg])
+  done
+
+lemma Afix_restr_subst:
+  assumes "x \<notin> S"
+  assumes "y \<notin> S"
+  assumes "domA \<Gamma> \<subseteq> S"
+  shows "Afix \<Gamma>[x::h=y]\<cdot>ae f|` S = Afix \<Gamma>\<cdot>(ae f|` S) f|` S"
+  by (rule Afix_restr_subst'[OF Aexp_subst_restr[OF assms(1,2)] assms])
+
+lemma Afix_comp2join_fresh:
+  "atom ` (domA \<Delta>) \<sharp>* \<Gamma> \<Longrightarrow> ABinds \<Delta>\<cdot>(Afix \<Gamma>\<cdot>ae) = Afix \<Gamma> \<cdot> ae \<squnion> ABinds \<Delta>\<cdot>ae"
+proof (induct \<Delta> rule: ABinds.induct)
+  case 1 show ?case by (simp add: Afix_above_arg del: fun_meet_simp)
+next
+  case (2 v e \<Delta>)
+  from 2(2)
+  have "atom v \<sharp> \<Gamma>" and  "atom ` domA (delete v \<Delta>) \<sharp>* \<Gamma>"
+    by (auto simp add: fresh_star_def)
+  from 2(1)[OF this(2)]
+  show ?case
+    by (simp del: fun_meet_simp add: Afix_lookup_fresh[OF `atom v \<sharp> \<Gamma>`])
+       (metis (hide_lams, no_types) join_assoc join_comm)
+qed
+
+lemma Afix_append_fresh:
+  assumes "atom ` domA \<Delta> \<sharp>* \<Gamma>"
+  shows "Afix (\<Delta> @ \<Gamma>)\<cdot>ae = Afix \<Gamma>\<cdot>(Afix \<Delta>\<cdot>ae)"
+proof (rule below_antisym)
+  show *: "Afix (\<Delta> @ \<Gamma>)\<cdot>ae \<sqsubseteq> Afix \<Gamma>\<cdot>(Afix \<Delta>\<cdot>ae)"
+  by (rule Afix_least_below)
+     (simp_all add:  Abinds_append_fresh[OF assms] Afix_comp2join_fresh[OF assms] Afix_above_arg below_trans[OF Afix_above_arg Afix_above_arg])
+next
+  show "Afix \<Gamma>\<cdot>(Afix \<Delta>\<cdot>ae) \<sqsubseteq> Afix (\<Delta> @ \<Gamma>)\<cdot>ae"
+  proof (rule Afix_least_below)
+    show "ABinds \<Gamma>\<cdot>(Afix (\<Delta> @ \<Gamma>)\<cdot>ae) \<sqsubseteq> Afix (\<Delta> @ \<Gamma>)\<cdot>ae"
+      apply (subst Abinds_Afix[symmetric]) back
+      apply (subst Abinds_append_fresh[OF assms])
+      apply (rule ABinds_above_arg)
+      done
+    show "Afix \<Delta>\<cdot>ae \<sqsubseteq> Afix (\<Delta> @ \<Gamma>)\<cdot>ae"
+      apply (rule Afix_least_below)
+      apply (subst Abinds_Afix[symmetric]) back
+      apply (subst Abinds_append_fresh[OF assms])
+      apply (rule monofun_cfun_arg[OF ABinds_above_arg])
+      apply (rule Afix_above_arg)
+      done
+  qed
+qed
+
+lemma Afix_e_to_heap:
+   "Afix (delete x \<Gamma>)\<cdot>(Aexp' e\<cdot>n \<squnion> ae) \<sqsubseteq> Afix ((x, e) # delete x \<Gamma>)\<cdot>(AE_singleton x\<cdot>n \<squnion> ae)"
+    apply (simp add: Afix_eq)
+    apply (rule fix_least_below, simp)
+    apply (intro join_below)
+    apply (subst fix_eq, simp) back apply (simp add: below_trans[OF _ join_above2])
+    apply (subst fix_eq, simp)
+    apply (rule below_trans[OF monofun_cfun_arg join_above1])
+    apply (subst fix_eq, simp)
+    apply (rule below_trans[OF _ join_above2])
+    apply (rule below_trans[OF _ join_above2])
+    apply simp
+    apply (subst fix_eq, simp)
+    apply (rule below_trans[OF _ join_above2])
+    apply (rule below_trans[OF _ join_above2])
+    apply (rule below_trans[OF _ join_above2])
+    apply simp
+    done
+
+lemma Afix_e_to_heap':
+   "Afix (delete x \<Gamma>)\<cdot>(Aexp e\<cdot>n) \<sqsubseteq> Afix ((x, e) # delete x \<Gamma>)\<cdot>(AE_singleton x\<cdot>(up\<cdot>n))"
+using Afix_e_to_heap[where ae = \<bottom> and n = "up\<cdot>n"] by simp
+
+end
+
+context CorrectArityAnalysisAfix
+begin
+lemma Aexp'_Let: "Afix as\<cdot>(Aexp' e\<cdot>n) f|` (- domA as) \<sqsubseteq> Aexp' (Terms.Let as e)\<cdot>n"
+  by (cases n) (simp_all add: Aexp_Let)
+
+lemma  reds_improves_arity':
+       "\<Gamma> : e \<Down>\<^bsub>L\<^esub> \<Delta> : v \<Longrightarrow>
+        edom ae \<subseteq> set L \<Longrightarrow> 
+        Afix \<Delta> \<cdot> (Aexp' v \<cdot> n \<squnion> ae) f|` (- (domA \<Delta> - domA \<Gamma>)) \<sqsubseteq> Afix \<Gamma> \<cdot> (Aexp' e \<cdot> n \<squnion> ae) f|` (- (domA \<Delta> - domA \<Gamma>))"
+proof(induct arbitrary: ae n rule: reds.induct)
+case Lambda
+  show ?case by simp
+next
+case (Variable \<Gamma> x e L \<Delta> z ae n)
+  have reorder: "map_of ((x, e) # delete x \<Gamma>) = map_of \<Gamma>" by (rule map_of_delete_insert[OF Variable.hyps(1)])
+
+  from `edom ae \<subseteq> set L`
+  have prem: "edom ae \<subseteq> set (x#L)" by auto
+
+  from `map_of \<Gamma> x = Some e` have [simp]: "x \<in> domA \<Gamma>" by (metis domA_from_set map_of_is_SomeD)
+
+  have "x \<notin> domA \<Delta>" by (rule reds_avoids_live[OF Variable(2), where x = x]) simp_all
+  hence [simp]:"delete x \<Delta> = \<Delta>" by simp
+
+  note IH =  Variable(3)
+  let "?S" = "(- (domA ((x, z) # \<Delta>) - domA \<Gamma>))"
+
+  have "Afix ((x, z) # \<Delta>) \<cdot> (Aexp' z\<cdot>n \<squnion> ae)  f|` ?S = (\<mu> ae'. Aexp' z\<cdot>(ae' x) \<squnion> ABinds \<Delta> \<cdot> ae' \<squnion> Aexp' z\<cdot>n \<squnion> ae) f|` ?S"
+    unfolding Afix_eq by simp
+  also have "\<dots> = (\<mu> ae'. ABinds \<Delta> \<cdot> ae' \<squnion> (Aexp' z\<cdot>n \<squnion> Aexp' z\<cdot>(ae' x) \<squnion> ae)) f|` ?S" by (metis (hide_lams, no_types) join_assoc join_comm)
+  also have "\<dots> \<sqsubseteq> (\<mu> ae'. ABinds \<Delta> \<cdot> ae' \<squnion> (Aexp' z\<cdot>(n \<squnion> ae' x) \<squnion> ae)) f|` ?S"
+    by (auto intro!: env_restr_mono monofun_cfun_arg cfun_belowI join_mono[OF below_refl] join_mono[OF _ below_refl] cfun_join_below simp del: join_assoc)
+  also have "\<dots> = (\<mu> ae'. Afix \<Delta> \<cdot> ae' \<squnion> (Aexp' z\<cdot>(n \<squnion> ae' x) \<squnion> ae))  f|` ?S"
+    apply (rule arg_cong[where f = "\<lambda> x. x f|` ?S"] )
+    apply (rule fix_eq_fix)
+    apply simp
+    apply (subst fix_eq) back back apply simp
+    apply (rule join_mono[OF _ below_refl])
+    apply (rule monofun_cfun_fun)
+    apply (rule Abinds_below_Afix)
+
+    apply simp
+    apply (rule join_below)
+    apply (subst Afix_eq)
+    apply (rule fix_least_below)
+    apply simp
+    apply (subst fix_eq) back apply simp
+    apply (subst fix_eq) back apply simp
+    done
+  also have "\<dots> = (\<mu> ae'. Afix \<Delta> \<cdot> (Aexp' z\<cdot>(n \<squnion> ae' x) \<squnion> ae)) f|` ?S"
+    apply (rule arg_cong[where f = "\<lambda> x. x f|` ?S"] )
+    apply (rule fix_eq_fix)
+    apply simp
+    apply (rule join_below)
+    apply (subst Afix_eq)
+    apply (rule fix_least_below, simp)
+    apply (subst (1 2) fix_eq, simp)
+    apply (subst fix_eq, simp)back
+    apply (rule Afix_above_arg)
+
+    apply simp
+    apply (subst fix_eq, simp) back
+    apply (rule below_trans[OF monofun_cfun_arg join_above1])
+    apply (rule join_below)
+    apply (subst fix_eq, simp) back
+    apply (rule below_trans[OF _ join_above2], simp)
+    
+    apply (subst fix_eq)  apply simp
+    apply (rule below_trans[OF _ join_above2], simp)
+    done
+    
+  also have "\<dots> \<sqsubseteq> (\<mu> ae'. Afix (delete x \<Gamma>) \<cdot> (Aexp' e\<cdot>(n \<squnion> ae' x) \<squnion> ae)) f|` ?S"
+  proof (induction rule: parallel_fix_ind[where P ="\<lambda> x y. x f|` ?S \<sqsubseteq> y f|` ?S"])
+  case (goal3 aeL aeR)
+    have "- (domA ((x, z) # \<Delta>) - domA \<Gamma>) \<subseteq> - (domA \<Delta> - domA (delete x \<Gamma>))"
+      using `x \<notin> domA \<Delta>` by auto
+    moreover
+    note IH[OF prem]
+    ultimately have "(Afix \<Delta>\<cdot>(Aexp' z\<cdot>(n \<squnion> aeL x) \<squnion> ae)) f|` ?S \<sqsubseteq> (Afix (delete x \<Gamma>)\<cdot>(Aexp' e\<cdot>(n \<squnion> aeL x) \<squnion> ae)) f|` ?S"
+      by (rule env_restr_below_subset)
+    also from goal3 have "aeL x \<sqsubseteq>  aeR x" by (rule env_restr_belowD) simp
+    finally have "Afix \<Delta>\<cdot>(Aexp' z\<cdot>(n \<squnion> aeL x) \<squnion> ae) f|` ?S \<sqsubseteq> Afix (delete x \<Gamma>)\<cdot>(Aexp' e\<cdot>(n \<squnion> aeR x) \<squnion> ae) f|` ?S" by this simp_all
+    thus ?case by simp
+  qed simp_all
+  also have "\<dots> \<sqsubseteq> (\<mu> ae'. Afix ((x,e)#delete x \<Gamma>) \<cdot> (AE_singleton x \<cdot> (n \<squnion> ae' x) \<squnion> ae))  f|` ?S"
+    apply (rule env_restr_mono)
+    apply (rule monofun_cfun_arg)
+    apply (rule cfun_belowI, simp)
+    apply (rule Afix_e_to_heap)
+    done
+  also have "\<dots> = Afix ((x,e)#delete x \<Gamma>) \<cdot> (AE_singleton x\<cdot>n \<squnion> ae)  f|` ?S" by (rule arg_cong[OF Afix_repeat_singleton])
+  also have "\<dots> \<sqsubseteq> Afix ((x,e)#delete x \<Gamma>) \<cdot> (Aexp' (Var x) \<cdot> n \<squnion> ae)  f|` ?S" by (intro Aexp'_Var monofun_cfun env_restr_mono join_mono below_refl)
+  also have "\<dots> = Afix \<Gamma> \<cdot> (Aexp' (Var x)\<cdot>n \<squnion> ae) f|` ?S" by (rule arg_cong[OF Afix_reorder[OF reorder]])
+  finally show "Afix ((x, z) # \<Delta>)\<cdot>(Aexp' z\<cdot>n \<squnion> ae) f|` ?S \<sqsubseteq> Afix \<Gamma>\<cdot>(Aexp' (Var x)\<cdot>n \<squnion> ae) f|` ?S"
+    by this simp_all
+next
+case (Application y \<Gamma> e x L \<Delta> \<Theta> z e' ae n)
+  note prem1 =  `edom ae \<subseteq> set L`
+  hence prem2: "edom ae \<subseteq> set (x#L)" by auto
+  hence prem3: "edom (AE_singleton x\<cdot>(up\<cdot>0) \<squnion> ae) \<subseteq> set (x#L)" by auto
+
+  have subset1: " (- (domA \<Theta> - domA \<Gamma>)) \<subseteq> (- (domA \<Theta> - domA \<Delta>))"
+    and subset2: "(- (domA \<Theta> - domA \<Gamma>)) \<subseteq> (- (domA \<Delta> - domA \<Gamma>))"
+    using reds_doesnt_forget[OF Application(2)]  reds_doesnt_forget[OF Application(4)] by auto
+  let "?S" = " (- (domA \<Theta> - domA \<Gamma>))"
+
+  show "Afix \<Theta>\<cdot>(Aexp' z\<cdot>n \<squnion> ae) f|` ?S \<sqsubseteq> Afix \<Gamma>\<cdot>(Aexp' (App e x)\<cdot>n \<squnion> ae)  f|` ?S"
+  proof(cases n)
+    case bottom
+    from env_restr_below_trans[OF env_restr_below_subset[OF subset1 Application(5)[OF prem1, where n = "\<bottom>"], simplified]
+                                  env_restr_below_subset[OF subset2 Application(3)[OF prem2, where n = "\<bottom>"], simplified]]
+    show ?thesis using bottom by simp
+  next
+    case (up n')
+    note IH1 = env_restr_below_subset[OF subset2 Application(3)[OF prem3, where n = "inc\<^sub>\<bottom>\<cdot>n"], unfolded up Aexp'_simps inc_bot_simps] 
+    note IH2 = env_restr_below_subset[OF subset1 Application(5)[OF prem1, where n = n], unfolded up Aexp'_simps]
+    have "Afix \<Theta>\<cdot>(Aexp z\<cdot>n' \<squnion> ae)  f|` ?S  \<sqsubseteq> Afix \<Delta>\<cdot>(Aexp e'[y::=x]\<cdot>n' \<squnion> ae)  f|` ?S" by (rule IH2)
+    also have "\<dots> \<sqsubseteq> Afix \<Delta>\<cdot>(Aexp (App (Lam [y]. e') x)\<cdot>n' \<squnion> ae) f|` ?S" by (intro monofun_cfun_arg monofun_cfun_fun env_restr_mono Aexp_subst_App_Lam join_mono below_refl)
+    also have "\<dots> = Afix \<Delta>\<cdot>(Aexp (Lam [y]. e')\<cdot>(inc\<cdot>n') \<squnion> AE_singleton x \<cdot> (up\<cdot>0) \<squnion> ae)  f|` ?S"  by (rule arg_cong[OF Aexp_App])
+    also have "\<dots> = Afix \<Delta>\<cdot>(Aexp (Lam [y]. e')\<cdot>(inc\<cdot>n') \<squnion> (AE_singleton x\<cdot>(up\<cdot>0) \<squnion> ae))  f|` ?S"  by simp
+    also have "\<dots> \<sqsubseteq> Afix \<Gamma>\<cdot>(Aexp e\<cdot>(inc\<cdot>n') \<squnion> (AE_singleton x\<cdot>(up\<cdot>0) \<squnion> ae)) f|` ?S" by (rule IH1)
+    also have "\<dots> = Afix \<Gamma>\<cdot>(Aexp e\<cdot>(inc\<cdot>n') \<squnion> AE_singleton x\<cdot>(up\<cdot>0) \<squnion> ae)  f|` ?S" by simp
+    also have "\<dots> = Afix \<Gamma>\<cdot>(Aexp (App e x)\<cdot>n' \<squnion> ae)  f|` ?S" by (rule arg_cong[OF Aexp_App[symmetric]])
+    finally
+    show ?thesis unfolding up by simp
+  qed
+next
+case (Let as \<Gamma> L e \<Delta> z ae n)
+  have *: "atom ` domA as \<sharp>* \<Gamma>" using Let(1) by (metis fresh_star_Pair)
+
+  let ?S = "(- (domA \<Delta> - domA \<Gamma>))"
+  have subset: "?S \<subseteq>  (- (domA \<Delta> - domA (as @ \<Gamma>)))" by auto
+
+  note prem = `edom ae \<subseteq> set L`
+  note IH = env_restr_below_subset[OF subset Let(3)[OF prem]]
+
+  from `atom \` domA as \<sharp>* (\<Gamma>, L)`
+  have "atom ` domA as \<sharp>* set L" by (auto simp add: fresh_star_Pair set_bn_to_atom_domA fresh_star_set)
+  hence "domA as \<inter> set L = {}" by (metis Int_commute disjoint_iff_not_equal fresh_list_elem fresh_set fresh_star_def image_eqI not_self_fresh)
+  with prem
+  have **: "ae ` domA as \<subseteq> {\<bottom>}" by (auto simp add: edom_def)
+
+  have [simp]: "ae f|` (-domA as) = ae" apply (rule env_restr_useless) using prem `domA as \<inter> set L = {}` by auto
+
+  from `atom \` domA as \<sharp>* \<Gamma>` have "domA as \<inter> domA \<Gamma> = {}" by (metis fresh_distinct)
+  moreover from reds_doesnt_forget[OF Let(2)] have "domA as \<subseteq> domA \<Delta>" by auto
+  ultimately have ***: "((- domA \<Delta> \<union> domA \<Gamma>) \<inter> - domA as) = (- domA \<Delta> \<union> domA \<Gamma>)" by auto
+
+  have "Afix \<Delta>\<cdot>(Aexp' z\<cdot>n \<squnion> ae)  f|` ?S \<sqsubseteq> Afix (as @ \<Gamma>)\<cdot>(Aexp' e\<cdot>n \<squnion> ae)  f|` ?S" by (rule IH)
+  also have "\<dots> = Afix \<Gamma>\<cdot>(Afix as\<cdot>(Aexp' e\<cdot>n \<squnion> ae))  f|` ?S" by (rule arg_cong[OF Afix_append_fresh[OF *]])
+  also have "\<dots> = Afix \<Gamma>\<cdot>(Afix as\<cdot>(Aexp' e\<cdot>n) \<squnion> ae)  f|` ?S" by (rule arg_cong[OF Afix_join_fresh[OF **]])
+  also have "\<dots> = Afix \<Gamma>\<cdot>(Afix as\<cdot>(Aexp' e\<cdot>n) \<squnion> ae) f|` (- (domA as)) f|` ?S" by (simp add: ***)
+  also have "\<dots> = Afix \<Gamma>\<cdot>((Afix as\<cdot>(Aexp' e\<cdot>n) \<squnion> ae) f|` (- (domA as))) f|` (- (domA as)) f|` ?S" by (rule arg_cong[OF Afix_restr_fresh[OF *]])
+  also have "\<dots> = Afix \<Gamma>\<cdot>((Afix as\<cdot>(Aexp' e\<cdot>n) \<squnion> ae) f|` (- (domA as))) f|` ?S" by (simp add: ***)
+  also have "\<dots> = Afix \<Gamma>\<cdot>((Afix as\<cdot>(Aexp' e\<cdot>n)  f|` (- (domA as))) \<squnion> ae) f|` ?S" by (simp add: env_restr_join)
+  also have "\<dots> \<sqsubseteq> Afix \<Gamma>\<cdot>(Aexp' (Terms.Let as e)\<cdot>n \<squnion> ae) f|` ?S" by (intro monofun_cfun_arg join_mono env_restr_mono below_refl Aexp'_Let)
+  finally
+  show "Afix \<Delta>\<cdot>(Aexp' z\<cdot>n \<squnion> ae) f|` ?S \<sqsubseteq> Afix \<Gamma>\<cdot>(Aexp' (Terms.Let as e)\<cdot>n \<squnion> ae) f|` ?S" by this simp_all
+qed
+
+corollary  reds_improves_arity'':
+       "\<Gamma> : e \<Down>\<^bsub>L\<^esub> \<Delta> : v \<Longrightarrow>
+        edom ae \<subseteq> set L \<Longrightarrow> 
+        Afix \<Delta> \<cdot> (Aexp v \<cdot> n \<squnion> ae) f|` (- (domA \<Delta> - domA \<Gamma>)) \<sqsubseteq> Afix \<Gamma> \<cdot> (Aexp e \<cdot> n \<squnion> ae) f|` (- (domA \<Delta> - domA \<Gamma>))"
+using reds_improves_arity'[OF assms, where n = "up\<cdot>n", simplified] by simp
+
+corollary  reds_improves_arity:
+  assumes "\<Gamma> : e \<Down>\<^bsub>L\<^esub> \<Delta> : v"
+  shows "Afix \<Delta> \<cdot> (Aexp' v \<cdot> n) f|` (- (domA \<Delta> - domA \<Gamma>)) \<sqsubseteq> Afix \<Gamma> \<cdot> (Aexp' e \<cdot> n) f|` (- (domA \<Delta> - domA \<Gamma>))"
+  using reds_improves_arity'[where ae = \<bottom>, OF assms] by simp
+end
+
+end
+
