Launchbury/ArityCorrect.thy
@@ -17,10 +17,6 @@ lemma ABinds_edom: "edom (ABinds \<Gamma> \<cdot> ae) \<subseteq> fv \<Gamma> \<
   apply (auto dest: set_mp[OF fv_delete_subset])
   done
 
-lemma Afix_edom: "edom (Afix \<Gamma> \<cdot> ae) \<subseteq> fv \<Gamma> \<union> edom ae"
-  unfolding Afix_eq
-  by (rule fix_ind[where P = "\<lambda> ae' . edom ae' \<subseteq> fv \<Gamma> \<union> edom ae"] )
-     (auto dest: set_mp[OF ABinds_edom])
 end
 
 locale CorrectArityAnalysis = EdomArityAnalysis +
@@ -30,9 +26,6 @@ locale CorrectArityAnalysis = EdomArityAnalysis +
   assumes Aexp_Lam: "Aexp (Lam [y]. e) \<cdot> n = env_delete y (Aexp e \<cdot>(pred\<cdot>n))"
   assumes Aexp_App: "Aexp (App e x) \<cdot> n = Aexp e \<cdot>(inc\<cdot>n) \<squnion> AE_singleton x \<cdot> (up\<cdot>0)"
   assumes Aexp_subst_restr: "x \<notin> S \<Longrightarrow> y \<notin> S \<Longrightarrow> (Aexp e[x::=y] \<cdot> a) f|` S = (Aexp e\<cdot>a) f|` S"
-
-locale CorrectArityAnalysisAfix = CorrectArityAnalysis + 
-  assumes Aexp_Let: "Afix as\<cdot>(Aexp e\<cdot>n) f|` (- domA as) \<sqsubseteq> Aexp (Let as e)\<cdot>n"
 
 locale CorrectArityAnalysisAheap = CorrectArityAnalysis + 
   fixes Aheap :: "heap \<Rightarrow> AEnv \<rightarrow> AEnv"
@@ -69,22 +62,6 @@ lemma ABinds_lookup_fresh:
   "atom v \<sharp> \<Gamma> \<Longrightarrow> (ABinds \<Gamma>\<cdot>ae) v = ae v"
 by (induct \<Gamma> rule: ABinds.induct) (auto simp add: fresh_Cons fresh_Pair Aexp'_lookup_fresh fresh_delete)
 
-lemma Afix_lookup_fresh:
-  assumes "atom v \<sharp> \<Gamma>"
-  shows "(Afix \<Gamma>\<cdot>ae) v = ae v"
-  apply (rule below_antisym)
-  apply (subst Afix_eq)
-  apply (rule fix_ind[where  P = "\<lambda> ae'. ae' v \<sqsubseteq> ae v"])
-  apply (auto simp add: ABinds_lookup_fresh[OF assms] fun_belowD[OF Afix_above_arg])
-  done
-
-lemma Afix_restr_subst:
-  assumes "x \<notin> S"
-  assumes "y \<notin> S"
-  assumes "domA \<Gamma> \<subseteq> S"
-  shows "Afix \<Gamma>[x::h=y]\<cdot>ae f|` S = Afix \<Gamma>\<cdot>(ae f|` S) f|` S"
-  by (rule Afix_restr_subst'[OF Aexp_subst_restr[OF assms(1,2)] assms])
-
 lemma Abinds_append_fresh: "atom ` (domA \<Delta>) \<sharp>* \<Gamma> \<Longrightarrow>  ABinds (\<Delta> @ \<Gamma>)\<cdot>ae = ABinds \<Delta>\<cdot>(ABinds \<Gamma>\<cdot>ae)"
 proof (induct \<Delta> rule: ABinds.induct)
   case 1 thus ?case by simp
@@ -103,243 +80,7 @@ next
   show "ABinds (((v, e) # \<Delta>) @ \<Gamma>)\<cdot>ae = ABinds ((v, e) # \<Delta>)\<cdot>(ABinds \<Gamma>\<cdot>ae)"
     by simp
 qed  
-
-lemma Afix_comp2join_fresh:
-  "atom ` (domA \<Delta>) \<sharp>* \<Gamma> \<Longrightarrow> ABinds \<Delta>\<cdot>(Afix \<Gamma>\<cdot>ae) = Afix \<Gamma> \<cdot> ae \<squnion> ABinds \<Delta>\<cdot>ae"
-proof (induct \<Delta> rule: ABinds.induct)
-  case 1 show ?case by (simp add: Afix_above_arg del: fun_meet_simp)
-next
-  case (2 v e \<Delta>)
-  from 2(2)
-  have "atom v \<sharp> \<Gamma>" and  "atom ` domA (delete v \<Delta>) \<sharp>* \<Gamma>"
-    by (auto simp add: fresh_star_def)
-  from 2(1)[OF this(2)]
-  show ?case
-    by (simp del: fun_meet_simp add: Afix_lookup_fresh[OF `atom v \<sharp> \<Gamma>`])
-       (metis (hide_lams, no_types) join_assoc join_comm)
-qed
-
-lemma Afix_append_fresh:
-  assumes "atom ` domA \<Delta> \<sharp>* \<Gamma>"
-  shows "Afix (\<Delta> @ \<Gamma>)\<cdot>ae = Afix \<Gamma>\<cdot>(Afix \<Delta>\<cdot>ae)"
-proof (rule below_antisym)
-  show *: "Afix (\<Delta> @ \<Gamma>)\<cdot>ae \<sqsubseteq> Afix \<Gamma>\<cdot>(Afix \<Delta>\<cdot>ae)"
-  by (rule Afix_least_below)
-     (simp_all add:  Abinds_append_fresh[OF assms] Afix_comp2join_fresh[OF assms] Afix_above_arg below_trans[OF Afix_above_arg Afix_above_arg])
-next
-  show "Afix \<Gamma>\<cdot>(Afix \<Delta>\<cdot>ae) \<sqsubseteq> Afix (\<Delta> @ \<Gamma>)\<cdot>ae"
-  proof (rule Afix_least_below)
-    show "ABinds \<Gamma>\<cdot>(Afix (\<Delta> @ \<Gamma>)\<cdot>ae) \<sqsubseteq> Afix (\<Delta> @ \<Gamma>)\<cdot>ae"
-      apply (subst Abinds_Afix[symmetric]) back
-      apply (subst Abinds_append_fresh[OF assms])
-      apply (rule ABinds_above_arg)
-      done
-    show "Afix \<Delta>\<cdot>ae \<sqsubseteq> Afix (\<Delta> @ \<Gamma>)\<cdot>ae"
-      apply (rule Afix_least_below)
-      apply (subst Abinds_Afix[symmetric]) back
-      apply (subst Abinds_append_fresh[OF assms])
-      apply (rule monofun_cfun_arg[OF ABinds_above_arg])
-      apply (rule Afix_above_arg)
-      done
-  qed
-qed
-
-lemma Afix_e_to_heap:
-   "Afix (delete x \<Gamma>)\<cdot>(Aexp' e\<cdot>n \<squnion> ae) \<sqsubseteq> Afix ((x, e) # delete x \<Gamma>)\<cdot>(AE_singleton x\<cdot>n \<squnion> ae)"
-    apply (simp add: Afix_eq)
-    apply (rule fix_least_below, simp)
-    apply (intro join_below)
-    apply (subst fix_eq, simp) back apply (simp add: below_trans[OF _ join_above2])
-    apply (subst fix_eq, simp)
-    apply (rule below_trans[OF monofun_cfun_arg join_above1])
-    apply (subst fix_eq, simp)
-    apply (rule below_trans[OF _ join_above2])
-    apply (rule below_trans[OF _ join_above2])
-    apply simp
-    apply (subst fix_eq, simp)
-    apply (rule below_trans[OF _ join_above2])
-    apply (rule below_trans[OF _ join_above2])
-    apply (rule below_trans[OF _ join_above2])
-    apply simp
-    done
-
-lemma Afix_e_to_heap':
-   "Afix (delete x \<Gamma>)\<cdot>(Aexp e\<cdot>n) \<sqsubseteq> Afix ((x, e) # delete x \<Gamma>)\<cdot>(AE_singleton x\<cdot>(up\<cdot>n))"
-using Afix_e_to_heap[where ae = \<bottom> and n = "up\<cdot>n"] by simp
 end
-
-context CorrectArityAnalysisAfix
-begin
-lemma Aexp'_Let: "Afix as\<cdot>(Aexp' e\<cdot>n) f|` (- domA as) \<sqsubseteq> Aexp' (Terms.Let as e)\<cdot>n"
-  by (cases n) (simp_all add: Aexp_Let)
-
-lemma  reds_improves_arity':
-       "\<Gamma> : e \<Down>\<^bsub>L\<^esub> \<Delta> : v \<Longrightarrow>
-        edom ae \<subseteq> set L \<Longrightarrow> 
-        Afix \<Delta> \<cdot> (Aexp' v \<cdot> n \<squnion> ae) f|` (- (domA \<Delta> - domA \<Gamma>)) \<sqsubseteq> Afix \<Gamma> \<cdot> (Aexp' e \<cdot> n \<squnion> ae) f|` (- (domA \<Delta> - domA \<Gamma>))"
-proof(induct arbitrary: ae n rule: reds.induct)
-case Lambda
-  show ?case by simp
-next
-case (Variable \<Gamma> x e L \<Delta> z ae n)
-  have reorder: "map_of ((x, e) # delete x \<Gamma>) = map_of \<Gamma>" by (rule map_of_delete_insert[OF Variable.hyps(1)])
-
-  from `edom ae \<subseteq> set L`
-  have prem: "edom ae \<subseteq> set (x#L)" by auto
-
-  from `map_of \<Gamma> x = Some e` have [simp]: "x \<in> domA \<Gamma>" by (metis domA_from_set map_of_is_SomeD)
-
-  have "x \<notin> domA \<Delta>" by (rule reds_avoids_live[OF Variable(2), where x = x]) simp_all
-  hence [simp]:"delete x \<Delta> = \<Delta>" by simp
-
-  note IH =  Variable(3)
-  let "?S" = "(- (domA ((x, z) # \<Delta>) - domA \<Gamma>))"
-
-  have "Afix ((x, z) # \<Delta>) \<cdot> (Aexp' z\<cdot>n \<squnion> ae)  f|` ?S = (\<mu> ae'. Aexp' z\<cdot>(ae' x) \<squnion> ABinds \<Delta> \<cdot> ae' \<squnion> Aexp' z\<cdot>n \<squnion> ae) f|` ?S"
-    unfolding Afix_eq by simp
-  also have "\<dots> = (\<mu> ae'. ABinds \<Delta> \<cdot> ae' \<squnion> (Aexp' z\<cdot>n \<squnion> Aexp' z\<cdot>(ae' x) \<squnion> ae)) f|` ?S" by (metis (hide_lams, no_types) join_assoc join_comm)
-  also have "\<dots> \<sqsubseteq> (\<mu> ae'. ABinds \<Delta> \<cdot> ae' \<squnion> (Aexp' z\<cdot>(n \<squnion> ae' x) \<squnion> ae)) f|` ?S"
-    by (auto intro!: env_restr_mono monofun_cfun_arg cfun_belowI join_mono[OF below_refl] join_mono[OF _ below_refl] cfun_join_below simp del: join_assoc)
-  also have "\<dots> = (\<mu> ae'. Afix \<Delta> \<cdot> ae' \<squnion> (Aexp' z\<cdot>(n \<squnion> ae' x) \<squnion> ae))  f|` ?S"
-    apply (rule arg_cong[where f = "\<lambda> x. x f|` ?S"] )
-    apply (rule fix_eq_fix)
-    apply simp
-    apply (subst fix_eq) back back apply simp
-    apply (rule join_mono[OF _ below_refl])
-    apply (rule monofun_cfun_fun)
-    apply (rule Abinds_below_Afix)
-
-    apply simp
-    apply (rule join_below)
-    apply (subst Afix_eq)
-    apply (rule fix_least_below)
-    apply simp
-    apply (subst fix_eq) back apply simp
-    apply (subst fix_eq) back apply simp
-    done
-  also have "\<dots> = (\<mu> ae'. Afix \<Delta> \<cdot> (Aexp' z\<cdot>(n \<squnion> ae' x) \<squnion> ae)) f|` ?S"
-    apply (rule arg_cong[where f = "\<lambda> x. x f|` ?S"] )
-    apply (rule fix_eq_fix)
-    apply simp
-    apply (rule join_below)
-    apply (subst Afix_eq)
-    apply (rule fix_least_below, simp)
-    apply (subst (1 2) fix_eq, simp)
-    apply (subst fix_eq, simp)back
-    apply (rule Afix_above_arg)
-
-    apply simp
-    apply (subst fix_eq, simp) back
-    apply (rule below_trans[OF monofun_cfun_arg join_above1])
-    apply (rule join_below)
-    apply (subst fix_eq, simp) back
-    apply (rule below_trans[OF _ join_above2], simp)
-    
-    apply (subst fix_eq)  apply simp
-    apply (rule below_trans[OF _ join_above2], simp)
-    done
-    
-  also have "\<dots> \<sqsubseteq> (\<mu> ae'. Afix (delete x \<Gamma>) \<cdot> (Aexp' e\<cdot>(n \<squnion> ae' x) \<squnion> ae)) f|` ?S"
-  proof (induction rule: parallel_fix_ind[where P ="\<lambda> x y. x f|` ?S \<sqsubseteq> y f|` ?S"])
-  case (goal3 aeL aeR)
-    have "- (domA ((x, z) # \<Delta>) - domA \<Gamma>) \<subseteq> - (domA \<Delta> - domA (delete x \<Gamma>))"
-      using `x \<notin> domA \<Delta>` by auto
-    moreover
-    note IH[OF prem]
-    ultimately have "(Afix \<Delta>\<cdot>(Aexp' z\<cdot>(n \<squnion> aeL x) \<squnion> ae)) f|` ?S \<sqsubseteq> (Afix (delete x \<Gamma>)\<cdot>(Aexp' e\<cdot>(n \<squnion> aeL x) \<squnion> ae)) f|` ?S"
-      by (rule env_restr_below_subset)
-    also from goal3 have "aeL x \<sqsubseteq>  aeR x" by (rule env_restr_belowD) simp
-    finally have "Afix \<Delta>\<cdot>(Aexp' z\<cdot>(n \<squnion> aeL x) \<squnion> ae) f|` ?S \<sqsubseteq> Afix (delete x \<Gamma>)\<cdot>(Aexp' e\<cdot>(n \<squnion> aeR x) \<squnion> ae) f|` ?S" by this simp_all
-    thus ?case by simp
-  qed simp_all
-  also have "\<dots> \<sqsubseteq> (\<mu> ae'. Afix ((x,e)#delete x \<Gamma>) \<cdot> (AE_singleton x \<cdot> (n \<squnion> ae' x) \<squnion> ae))  f|` ?S"
-    apply (rule env_restr_mono)
-    apply (rule monofun_cfun_arg)
-    apply (rule cfun_belowI, simp)
-    apply (rule Afix_e_to_heap)
-    done
-  also have "\<dots> = Afix ((x,e)#delete x \<Gamma>) \<cdot> (AE_singleton x\<cdot>n \<squnion> ae)  f|` ?S" by (rule arg_cong[OF Afix_repeat_singleton])
-  also have "\<dots> \<sqsubseteq> Afix ((x,e)#delete x \<Gamma>) \<cdot> (Aexp' (Var x) \<cdot> n \<squnion> ae)  f|` ?S" by (intro Aexp'_Var monofun_cfun env_restr_mono join_mono below_refl)
-  also have "\<dots> = Afix \<Gamma> \<cdot> (Aexp' (Var x)\<cdot>n \<squnion> ae) f|` ?S" by (rule arg_cong[OF Afix_reorder[OF reorder]])
-  finally show "Afix ((x, z) # \<Delta>)\<cdot>(Aexp' z\<cdot>n \<squnion> ae) f|` ?S \<sqsubseteq> Afix \<Gamma>\<cdot>(Aexp' (Var x)\<cdot>n \<squnion> ae) f|` ?S"
-    by this simp_all
-next
-case (Application y \<Gamma> e x L \<Delta> \<Theta> z e' ae n)
-  note prem1 =  `edom ae \<subseteq> set L`
-  hence prem2: "edom ae \<subseteq> set (x#L)" by auto
-  hence prem3: "edom (AE_singleton x\<cdot>(up\<cdot>0) \<squnion> ae) \<subseteq> set (x#L)" by auto
-
-  have subset1: " (- (domA \<Theta> - domA \<Gamma>)) \<subseteq> (- (domA \<Theta> - domA \<Delta>))"
-    and subset2: "(- (domA \<Theta> - domA \<Gamma>)) \<subseteq> (- (domA \<Delta> - domA \<Gamma>))"
-    using reds_doesnt_forget[OF Application(2)]  reds_doesnt_forget[OF Application(4)] by auto
-  let "?S" = " (- (domA \<Theta> - domA \<Gamma>))"
-
-  show "Afix \<Theta>\<cdot>(Aexp' z\<cdot>n \<squnion> ae) f|` ?S \<sqsubseteq> Afix \<Gamma>\<cdot>(Aexp' (App e x)\<cdot>n \<squnion> ae)  f|` ?S"
-  proof(cases n)
-    case bottom
-    from env_restr_below_trans[OF env_restr_below_subset[OF subset1 Application(5)[OF prem1, where n = "\<bottom>"], simplified]
-                                  env_restr_below_subset[OF subset2 Application(3)[OF prem2, where n = "\<bottom>"], simplified]]
-    show ?thesis using bottom by simp
-  next
-    case (up n')
-    note IH1 = env_restr_below_subset[OF subset2 Application(3)[OF prem3, where n = "inc\<^sub>\<bottom>\<cdot>n"], unfolded up Aexp'_simps inc_bot_simps] 
-    note IH2 = env_restr_below_subset[OF subset1 Application(5)[OF prem1, where n = n], unfolded up Aexp'_simps]
-    have "Afix \<Theta>\<cdot>(Aexp z\<cdot>n' \<squnion> ae)  f|` ?S  \<sqsubseteq> Afix \<Delta>\<cdot>(Aexp e'[y::=x]\<cdot>n' \<squnion> ae)  f|` ?S" by (rule IH2)
-    also have "\<dots> \<sqsubseteq> Afix \<Delta>\<cdot>(Aexp (App (Lam [y]. e') x)\<cdot>n' \<squnion> ae) f|` ?S" by (intro monofun_cfun_arg monofun_cfun_fun env_restr_mono Aexp_subst_App_Lam join_mono below_refl)
-    also have "\<dots> = Afix \<Delta>\<cdot>(Aexp (Lam [y]. e')\<cdot>(inc\<cdot>n') \<squnion> AE_singleton x \<cdot> (up\<cdot>0) \<squnion> ae)  f|` ?S"  by (rule arg_cong[OF Aexp_App])
-    also have "\<dots> = Afix \<Delta>\<cdot>(Aexp (Lam [y]. e')\<cdot>(inc\<cdot>n') \<squnion> (AE_singleton x\<cdot>(up\<cdot>0) \<squnion> ae))  f|` ?S"  by simp
-    also have "\<dots> \<sqsubseteq> Afix \<Gamma>\<cdot>(Aexp e\<cdot>(inc\<cdot>n') \<squnion> (AE_singleton x\<cdot>(up\<cdot>0) \<squnion> ae)) f|` ?S" by (rule IH1)
-    also have "\<dots> = Afix \<Gamma>\<cdot>(Aexp e\<cdot>(inc\<cdot>n') \<squnion> AE_singleton x\<cdot>(up\<cdot>0) \<squnion> ae)  f|` ?S" by simp
-    also have "\<dots> = Afix \<Gamma>\<cdot>(Aexp (App e x)\<cdot>n' \<squnion> ae)  f|` ?S" by (rule arg_cong[OF Aexp_App[symmetric]])
-    finally
-    show ?thesis unfolding up by simp
-  qed
-next
-case (Let as \<Gamma> L e \<Delta> z ae n)
-  have *: "atom ` domA as \<sharp>* \<Gamma>" using Let(1) by (metis fresh_star_Pair)
-
-  let ?S = "(- (domA \<Delta> - domA \<Gamma>))"
-  have subset: "?S \<subseteq>  (- (domA \<Delta> - domA (as @ \<Gamma>)))" by auto
-
-  note prem = `edom ae \<subseteq> set L`
-  note IH = env_restr_below_subset[OF subset Let(3)[OF prem]]
-
-  from `atom \` domA as \<sharp>* (\<Gamma>, L)`
-  have "atom ` domA as \<sharp>* set L" by (auto simp add: fresh_star_Pair set_bn_to_atom_domA fresh_star_set)
-  hence "domA as \<inter> set L = {}" by (metis Int_commute disjoint_iff_not_equal fresh_list_elem fresh_set fresh_star_def image_eqI not_self_fresh)
-  with prem
-  have **: "ae ` domA as \<subseteq> {\<bottom>}" by (auto simp add: edom_def)
-
-  have [simp]: "ae f|` (-domA as) = ae" apply (rule env_restr_useless) using prem `domA as \<inter> set L = {}` by auto
-
-  from `atom \` domA as \<sharp>* \<Gamma>` have "domA as \<inter> domA \<Gamma> = {}" by (metis fresh_distinct)
-  moreover from reds_doesnt_forget[OF Let(2)] have "domA as \<subseteq> domA \<Delta>" by auto
-  ultimately have ***: "((- domA \<Delta> \<union> domA \<Gamma>) \<inter> - domA as) = (- domA \<Delta> \<union> domA \<Gamma>)" by auto
-
-  have "Afix \<Delta>\<cdot>(Aexp' z\<cdot>n \<squnion> ae)  f|` ?S \<sqsubseteq> Afix (as @ \<Gamma>)\<cdot>(Aexp' e\<cdot>n \<squnion> ae)  f|` ?S" by (rule IH)
-  also have "\<dots> = Afix \<Gamma>\<cdot>(Afix as\<cdot>(Aexp' e\<cdot>n \<squnion> ae))  f|` ?S" by (rule arg_cong[OF Afix_append_fresh[OF *]])
-  also have "\<dots> = Afix \<Gamma>\<cdot>(Afix as\<cdot>(Aexp' e\<cdot>n) \<squnion> ae)  f|` ?S" by (rule arg_cong[OF Afix_join_fresh[OF **]])
-  also have "\<dots> = Afix \<Gamma>\<cdot>(Afix as\<cdot>(Aexp' e\<cdot>n) \<squnion> ae) f|` (- (domA as)) f|` ?S" by (simp add: ***)
-  also have "\<dots> = Afix \<Gamma>\<cdot>((Afix as\<cdot>(Aexp' e\<cdot>n) \<squnion> ae) f|` (- (domA as))) f|` (- (domA as)) f|` ?S" by (rule arg_cong[OF Afix_restr_fresh[OF *]])
-  also have "\<dots> = Afix \<Gamma>\<cdot>((Afix as\<cdot>(Aexp' e\<cdot>n) \<squnion> ae) f|` (- (domA as))) f|` ?S" by (simp add: ***)
-  also have "\<dots> = Afix \<Gamma>\<cdot>((Afix as\<cdot>(Aexp' e\<cdot>n)  f|` (- (domA as))) \<squnion> ae) f|` ?S" by (simp add: env_restr_join)
-  also have "\<dots> \<sqsubseteq> Afix \<Gamma>\<cdot>(Aexp' (Terms.Let as e)\<cdot>n \<squnion> ae) f|` ?S" by (intro monofun_cfun_arg join_mono env_restr_mono below_refl Aexp'_Let)
-  finally
-  show "Afix \<Delta>\<cdot>(Aexp' z\<cdot>n \<squnion> ae) f|` ?S \<sqsubseteq> Afix \<Gamma>\<cdot>(Aexp' (Terms.Let as e)\<cdot>n \<squnion> ae) f|` ?S" by this simp_all
-qed
-
-corollary  reds_improves_arity'':
-       "\<Gamma> : e \<Down>\<^bsub>L\<^esub> \<Delta> : v \<Longrightarrow>
-        edom ae \<subseteq> set L \<Longrightarrow> 
-        Afix \<Delta> \<cdot> (Aexp v \<cdot> n \<squnion> ae) f|` (- (domA \<Delta> - domA \<Gamma>)) \<sqsubseteq> Afix \<Gamma> \<cdot> (Aexp e \<cdot> n \<squnion> ae) f|` (- (domA \<Delta> - domA \<Gamma>))"
-using reds_improves_arity'[OF assms, where n = "up\<cdot>n", simplified] by simp
-
-corollary  reds_improves_arity:
-  assumes "\<Gamma> : e \<Down>\<^bsub>L\<^esub> \<Delta> : v"
-  shows "Afix \<Delta> \<cdot> (Aexp' v \<cdot> n) f|` (- (domA \<Delta> - domA \<Gamma>)) \<sqsubseteq> Afix \<Gamma> \<cdot> (Aexp' e \<cdot> n) f|` (- (domA \<Delta> - domA \<Gamma>))"
-  using reds_improves_arity'[where ae = \<bottom>, OF assms] by simp
-end
-
 
 (*
 context CorrectArityAnalysisAfix 
