Launchbury/CoCallAnalysis.thy
@@ -1,0 +1,10 @@
+theory CoCallAnalysis
+imports Terms "Arity-Nominal" CoCallGraph
+begin
+
+locale CoCallAnalysis =
+  fixes ccExp :: "exp \<Rightarrow> Arity \<rightarrow> CoCalls"
+  assumes "ccField (ccExp e\<cdot>a) \<subseteq> fv e"
+
+
+end
