Launchbury/CoCallGraph.thy
@@ -1,0 +1,26 @@
+theory CoCallGraph
+imports Main Vars HOLCF
+begin
+
+typedef CoCalls = "UNIV :: (var \<times> var) set set"
+  morphisms Rep_CoCall Abs_CoCall
+  by auto
+
+setup_lifting type_definition_CoCalls
+
+instantiation CoCalls :: po
+begin
+lift_definition below_CoCalls :: "CoCalls \<Rightarrow> CoCalls \<Rightarrow> bool" is "op \<subseteq>".
+instance
+  apply default
+  apply ((transfer, auto)+)
+  done
+end
+
+instance CoCalls :: cpo
+  sorry
+
+
+lift_definition ccField :: "CoCalls \<Rightarrow> var set" is Field.
+
+end
