Launchbury/TrivialArityAnal.thy
@@ -1,9 +1,15 @@
 theory TrivialArityAnal
-imports ArityCorrect
+imports ArityCorrect "Arity-Nominal" "Env-Nominal"
 begin
 
 definition Trivial_Aexp :: "exp \<Rightarrow> Arity \<rightarrow> AEnv"
   where "Trivial_Aexp e = (\<Lambda> n. (\<lambda> x. up\<cdot>0) f|` fv e)"
+
+lemma Trivial_Aexp_eqvt[eqvt]: "\<pi> \<bullet>  (Trivial_Aexp e) = Trivial_Aexp (\<pi> \<bullet> e)"
+  unfolding Trivial_Aexp_def
+  apply perm_simp
+  apply (simp add: Abs_cfun_eqvt)
+  done
 
 lemma Trivial_Aexp_simp: "Trivial_Aexp e \<cdot> n = (\<lambda> x. up\<cdot>0) f|` fv e"
   unfolding Trivial_Aexp_def by simp
@@ -11,6 +17,11 @@ lemma Trivial_Aexp_simp: "Trivial_Aexp e \<cdot> n = (\<lambda> x. up\<cdot>0) f
 lemma edom_Trivial_Aexp[simp]: "edom (Trivial_Aexp e \<cdot> n) = fv e"
   by (auto simp add: edom_def env_restr_def Trivial_Aexp_def) 
 
+lemma Trivial_Aexp_eq[iff]: "Trivial_Aexp e \<cdot> n = Trivial_Aexp e' \<cdot> n' \<longleftrightarrow> fv e = (fv e' :: var set)"
+  apply (auto simp add: Trivial_Aexp_simp env_restr_def)
+  apply (metis up_defined)+
+  done
+  
 lemma below_Trivial_Aexp[simp]: "(ae \<sqsubseteq> Trivial_Aexp e \<cdot> n) \<longleftrightarrow> edom ae \<subseteq> fv e"
   by (auto dest:fun_belowD intro!: fun_belowI  simp add: Trivial_Aexp_def env_restr_def edom_def split:if_splits)
 
@@ -21,6 +32,13 @@ interpretation EdomArityAnalysis Trivial_Aexp  by default simp
 
 interpretation CorrectArityAnalysis Trivial_Aexp
 proof default
+  fix \<pi>
+  show "\<pi> \<bullet> Trivial_Aexp = Trivial_Aexp" by perm_simp rule
+next
+  fix n x
+  show "up\<cdot>n \<sqsubseteq> (Trivial_Aexp (Var x)\<cdot>n) x"
+    by (simp add: Trivial_Aexp_simp)
+next
   fix e' y x
   show "Trivial_Aexp e'[y::=x] \<sqsubseteq> Trivial_Aexp (App (Lam [y]. e') x)"
     by (fastforce intro: cfun_belowI env_restr_mono2 dest: set_mp[OF fv_subst_subset])
@@ -29,12 +47,15 @@ next
   show "Trivial_Aexp (App e x)\<cdot>n = Trivial_Aexp e\<cdot>(inc\<cdot>n) \<squnion> AE_singleton x\<cdot>(up\<cdot>0)"
     by (auto simp add: Trivial_Aexp_def env_restr_def )
 next
-  fix as e n
-  show "Afix as\<cdot>(Trivial_Aexp e\<cdot>n) f|` (- domA as) \<sqsubseteq> Trivial_Aexp (Terms.Let as e)\<cdot>n"
-  by (auto dest: set_mp[OF Afix_edom])
+  fix y e n
+  show "Trivial_Aexp (Lam [y]. e)\<cdot>n = env_delete y (Trivial_Aexp e\<cdot>(pred\<cdot>n))"
+    by (auto simp add: Trivial_Aexp_simp env_delete_restr Diff_eq inf_commute)
 next
-  fix n x
-  show "up\<cdot>n \<sqsubseteq> (Trivial_Aexp (Var x)\<cdot>n) x"
-    by (simp add: Trivial_Aexp_def)
+  fix x y :: var and S e a
+  assume "x \<notin> S" and "y \<notin> S"
+  thus "Trivial_Aexp e[x::=y]\<cdot>a f|` S = Trivial_Aexp e\<cdot>a f|` S"
+    by (auto simp add: Trivial_Aexp_simp fv_subst_eq intro!: arg_cong[where f = "\<lambda> S. env_restr S e" for e])
 qed
+
+end
 
